handling or

coq/examples/test_19.c
@@ -1,0 +1,27 @@
+#include <stdlib.h>
+#include <stdbool.h>
+#include <stdint.h>
+#include <assert.h>
+
+#include <klee/klee.h>
+
+void f1(unsigned x) {
+    unsigned y = x | 10;
+}
+
+void f2() {
+    unsigned x = klee_make_symbolic_int32();
+    unsigned y = x | 10;
+}
+
+void f3() {
+    unsigned x = klee_make_symbolic_int32();
+    unsigned y = 10 | x;
+}
+
+int main() {
+    f1(100);
+    f2();
+    f3();
+    return 0;
+}
